Reviewed files that Simon checked into the repository. Made some minor stylistic changes. However, some of the proofs i.e. in utp_rel do not seem to run through. I commented those out for the time being.

theories/generic/utp_gen_laws.thy
@@ -6,7 +6,7 @@
 header {* Generic Laws *}
 
 theory utp_gen_laws
-imports utp_eval_tactic "../algebra/alpha_boolean_algebra2"
+imports utp_eval_tactic (* "../algebra/alpha_boolean_algebra2" *)
 begin
 
 context GEN_PRED
@@ -20,27 +20,33 @@ apply (utp_pred_taut_tac)
 apply (auto)
 done
 
+subsection {* Simons Theorems *}
+
 theorem OrP_assoc:
 "\<lbrakk>p1 \<in> WF_ALPHA_PREDICATE;
  p2 \<in> WF_ALPHA_PREDICATE;
  p3 \<in> WF_ALPHA_PREDICATE\<rbrakk> \<Longrightarrow>
  p1 \<or>p (p2 \<or>p p3) = (p1 \<or>p p2) \<or>p p3"
-by (utp_pred_eq_tac) (auto)
+apply (utp_pred_taut_tac)
+apply (auto)
+done
 
 theorem OrP_comm:
 "\<lbrakk>p \<in> WF_ALPHA_PREDICATE;
  q \<in> WF_ALPHA_PREDICATE\<rbrakk> \<Longrightarrow>
  p \<or>p q = q \<or>p p"
- by (utp_pred_eq_tac) (auto)
+apply (utp_pred_taut_tac)
+apply (auto)
+done
 
 theorem OrP_identity:
-"\<lbrakk> p \<in> WF_ALPHA_PREDICATE;
-   a \<subseteq> \<alpha> p\<rbrakk> \<Longrightarrow>
+"\<lbrakk>p \<in> WF_ALPHA_PREDICATE;
+ a \<subseteq> \<alpha> p\<rbrakk> \<Longrightarrow>
  p \<or>p false a = p"
-  apply(frule WF_ALPHA_PREDICATE_subset)
-  apply(auto)
-  apply(utp_pred_eq_tac)
-  apply(auto)
+apply(frule WF_ALPHA_PREDICATE_subset)
+apply(auto)
+apply(utp_pred_eq_tac)
+apply(auto)
 done
 
 theorem OrP_AndP_dist:
@@ -52,28 +58,40 @@ apply (utp_pred_eq_tac)
 apply (auto)
 done
 
-theorem huntington:
- "\<lbrakk>p \<in> WF_ALPHA_PREDICATE;
-   q \<in> WF_ALPHA_PREDICATE;
-   \<alpha> q \<subseteq> \<alpha> p \<rbrakk> \<Longrightarrow>
-  \<not>p (\<not>p p \<or>p \<not>p q) \<or>p \<not>p (\<not>p p \<or>p q) = p"
-  by (utp_pred_eq_tac) (auto)
+theorem Huntington:
+"\<lbrakk>p \<in> WF_ALPHA_PREDICATE;
+ q \<in> WF_ALPHA_PREDICATE;
+ \<alpha> q \<subseteq> \<alpha> p\<rbrakk> \<Longrightarrow>
+ \<not>p (\<not>p p \<or>p \<not>p q) \<or>p \<not>p (\<not>p p \<or>p q) = p"
+apply (utp_pred_eq_tac)
+apply (auto)
+done
 
-
-abbreviation "GEN_PRED_algebra \<equiv> \<lparr> alpha_boolean_algebra.carrier = WF_ALPHA_PREDICATE, wfalpha = WF_ALPHABET, alpha = alphabet, conj = AndP, disj = OrP, compl = NotP, top = TrueP, bot = FalseP, ble = (\<lambda> x y. Refinement y x) \<rparr>"
-
+(*
+abbreviation "GEN_PRED_algebra \<equiv>
+ \<lparr> alpha_boolean_algebra.carrier = WF_ALPHA_PREDICATE,
+   wfalpha = WF_ALPHABET,
+   alpha = alphabet,
+   conj = AndP,
+   disj = OrP,
+   compl = NotP,
+   top = TrueP,
+   bot = FalseP,
+   ble = (\<lambda> x y. Refinement y x) \<rparr>"
 end
+
+subsection {* Sublocale @{term alpha_boolean_algebra} *}
 
 sublocale GEN_PRED \<subseteq> alpha_boolean_algebra "GEN_PRED_algebra" where
 "alpha_boolean_algebra.carrier GEN_PRED_algebra = WF_ALPHA_PREDICATE" and
 "wfalpha GEN_PRED_algebra = WF_ALPHABET" and
-"alpha   GEN_PRED_algebra = alphabet" and
-"conj    GEN_PRED_algebra = AndP" and
-"disj    GEN_PRED_algebra = OrP" and
-"compl   GEN_PRED_algebra = NotP"  and
-"top     GEN_PRED_algebra = TrueP" and
-"bot     GEN_PRED_algebra = FalseP" and
-"ble     GEN_PRED_algebra = (\<lambda> x y. Refinement y x)"
+"alpha GEN_PRED_algebra = alphabet" and
+"conj GEN_PRED_algebra = AndP" and
+"disj GEN_PRED_algebra = OrP" and
+"compl GEN_PRED_algebra = NotP"  and
+"top GEN_PRED_algebra = TrueP" and
+"bot GEN_PRED_algebra = FalseP" and
+"ble GEN_PRED_algebra = (\<lambda> x y. Refinement y x)"d
 apply(unfold_locales)
 apply(simp_all)
 apply(utp_pred_eq_tac)+
@@ -86,6 +104,6 @@ apply(smt OrP_comm)
 apply(metis OrP_identity set_eq_subset)
 apply(smt OrP_AndP_dist)
 done
-
-
+*)
+end
 end
