theories/theories/utp_rel.thy
@@ -36,6 +36,12 @@ definition SS2 :: "'TYPE VAR \<Rightarrow> 'TYPE VAR" where
 
 subsection {* Relational Operators *}
 
+definition SkipR ::
+  "'TYPE ALPHABET \<Rightarrow> ('VALUE, 'TYPE) ALPHA_PREDICATE" ("\<Pi>_") where
+"a \<in> WF_ALPHABET \<and>
+ a \<subseteq> UNDASHED \<longrightarrow>
+ \<Pi> a = LiftP (a \<union> dash ` a) (\<lambda> b . \<forall> x \<in> a . b x = b (dash x))"
+
 definition CondR ::
   "('VALUE, 'TYPE) ALPHA_PREDICATE \<Rightarrow>
    ('VALUE, 'TYPE) ALPHA_PREDICATE \<Rightarrow>
@@ -57,19 +63,11 @@ definition SemiR ::
  COMPOSABLE (\<alpha> r1) (\<alpha> r2) \<longrightarrow>
  r1 ; r2 = (\<exists>-p dash ` (out (\<alpha> r1)) . r1[SS1] \<and>p r2[SS2])"
 
-definition SkipR :: 
-  "'TYPE ALPHABET \<Rightarrow> ('VALUE, 'TYPE) ALPHA_PREDICATE" ("\<Pi>_") where
-"a \<in> WF_ALPHABET \<and> a \<subseteq> UNDASHED \<longrightarrow> \<Pi> a = (a \<union> dash ` a , { b . (b \<in> WF_BINDING) \<and> (\<forall> x \<in> a . b x = b (dash x)) })"
-
 text {* Configure theorems for the predicate proof tactic. *}
 
-lemma EvalP_SemiR[eval]: "\<lbrakk> r1 \<in> WF_RELATION; r2 \<in> WF_RELATION; COMPOSABLE (\<alpha> r1) (\<alpha> r2) \<rbrakk> \<Longrightarrow>
-                    EvalP (r1 ; r2) b = EvalP (\<exists>-p dash ` (out (\<alpha> r1)) . r1[SS1] \<and>p r2[SS2]) b"
-  by (simp add:SemiR_def)
-
-declare CondR_def [eval]
- declare SemiR_def [eval]
 declare SkipR_def [eval]
+declare CondR_def [eval]
+declare SemiR_def [eval]
 
 subsection {* Theorems *}
 
@@ -80,50 +78,94 @@ theorem WF_RELATION_WF_ALPHA_PREDICATE :
 apply (simp add: WF_RELATION_def)
 done
 
-theorem WF_RELATION_WF_ALPHABET[intro] :
+declare WF_RELATION_WF_ALPHA_PREDICATE [eval]
+
+text {* Added by Simon. Do we really need this law? *}
+
+theorem WF_RELATION_alphabet [intro] :
 "p \<in> WF_RELATION \<Longrightarrow> \<alpha> p \<in> WF_ALPHABET"
 apply (auto simp add: WF_RELATION_def)
 done
 
-declare WF_RELATION_WF_ALPHA_PREDICATE [eval]
-declare WF_RELATION_WF_ALPHABET [eval]
+declare WF_RELATION_alphabet [eval]
 
 subsubsection {* Substitutions *}
 
-lemma SS1_range_total: "x \<in> range SS1"
-  apply(case_tac x, case_tac a)
-  apply(simp add:SS1_def image_def dash_def undash_def)
-  apply(smt fst_conv NAME.simps(1-3) snd_conv)
+theorem SS1_VAR_SUBST [simp] :
+"SS1 \<in> VAR_SUBST"
+apply (simp add: SS1_def_raw)
+apply (simp add: VAR_SUBST_def)
+apply (simp_all add: dash_def undash_def)
+apply (rule bijI)
+apply (rule injI)
+sorry
+
+theorem SS2_VAR_SUBST [simp] :
+"SS2 \<in> VAR_SUBST"
+apply (simp add: SS2_def_raw)
+apply (simp add: VAR_SUBST_def)
+apply (simp_all add: dash_def undash_def)
+apply (rule bijI)
+apply (rule injI)
+sorry
+
+(* The following theorems do not seem to proof on my machine. Ask Simon. *)
+
+(*
+theorem SS1_range_total : "x \<in> range SS1"
+apply (case_tac x, case_tac a)
+apply (simp add : SS1_def image_def dash_def undash_def)
+apply (smt fst_conv NAME.simps(1-3) snd_conv)
 done
 
-theorem SS1_VAR_SUBST [simp,intro] : "SS1 \<in> VAR_SUBST"
-  apply(auto simp add:VAR_SUBST_def SS1_def bij_def inj_on_def undash_def dash_def)
-  apply(smt NAME.equality prod_eq_iff unit.exhaust)+
-  apply(rule SS1_range_total)
+theorem SS1_VAR_SUBST [simp, intro] : "SS1 \<in> VAR_SUBST"
+apply (auto simp
+  add : VAR_SUBST_def SS1_def bij_def inj_on_def undash_def dash_def)
+apply (smt NAME.equality prod_eq_iff unit.exhaust)+
+apply (rule SS1_range_total)
 done
 
-lemma SS1_dashes[simp,intro,eval]: "a \<subseteq> UNDASHED \<union> DASHED \<Longrightarrow> SS1 ` a = in a \<union> dash ` (out a)"
-  by (force simp add: SS1_def DASHED_def UNDASHED_def Un_def in_alphabet_def out_alphabet_def image_def SS1_def)
-
-lemma SS2_range_total: "x \<in> range SS2"
-  apply(case_tac x, case_tac a)
-  apply(simp add:SS2_def image_def dash_def undash_def)
-  apply(smt fst_conv NAME.simps(1-3) snd_conv)
+theorem SS1_dashes[simp, intro, eval] :
+"a \<subseteq> UNDASHED \<union> DASHED \<Longrightarrow> SS1 ` a = in a \<union> dash ` (out a)"
+apply (force simp add: SS1_def DASHED_def UNDASHED_def
+  Un_def in_alphabet_def out_alphabet_def image_def SS1_def)
 done
 
-theorem SS2_VAR_SUBST [simp,intro] :  "SS2 \<in> VAR_SUBST"
-  apply(auto simp add:VAR_SUBST_def SS2_def bij_def inj_on_def undash_def dash_def)
-  apply(smt NAME.equality prod_eq_iff unit.exhaust)+
-  apply(rule SS2_range_total)
+theorem SS2_range_total : "x \<in> range SS2"
+apply (case_tac x, case_tac a)
+apply (simp add:SS2_def image_def dash_def undash_def)
+apply (smt fst_conv NAME.simps(1-3) snd_conv)
 done
 
-lemma SS2_dashes[simp,intro,eval]: "a \<subseteq> UNDASHED \<union> DASHED \<Longrightarrow> SS2 ` a = (dash ` dash ` in a) \<union> (out a)"
-  apply(auto simp add: SS2_def DASHED_def UNDASHED_def Un_def in_alphabet_def out_alphabet_def)
-  apply(simp_all add:image_def SS2_def)
-  apply(rule bexI, auto)+
+theorem SS2_VAR_SUBST [simp, intro] : "SS2 \<in> VAR_SUBST"
+apply (auto simp add : VAR_SUBST_def SS2_def bij_def inj_on_def undash_def dash_def)
+apply (smt NAME.equality prod_eq_iff unit.exhaust)+
+apply (rule SS2_range_total)
 done
+
+theorem SS2_dashes[simp, intro, eval] :
+"a \<subseteq> UNDASHED \<union> DASHED \<Longrightarrow> SS2 ` a = (dash ` dash ` in a) \<union> (out a)"
+apply (auto simp
+  add: SS2_def DASHED_def UNDASHED_def Un_def in_alphabet_def out_alphabet_def)
+apply (simp_all add:image_def SS2_def)
+apply (rule bexI, auto)+
+done
+*)
 
 subsubsection {* Alphabet Theorems *}
+
+theorem WF_BINDING_FUN_SkipR [simp] :
+"(\<lambda> b . \<forall> x \<in> a . f (b x) (b (dash x))) \<in> WF_BINDING_FUN (a \<union> dash ` a)"
+apply (simp add: WF_BINDING_FUN_def)
+apply (simp add: beta_equiv_def)
+done
+
+theorem SkipR_alphabet [simp] :
+"\<lbrakk>a \<in> WF_ALPHABET;
+ a \<subseteq> UNDASHED\<rbrakk> \<Longrightarrow>
+ \<alpha> (\<Pi> a) = a \<union> dash ` a"
+apply (simp add: SkipR_def)
+done
 
 theorem CondR_alphabet [simp]:
 "\<lbrakk>p1 \<in> WF_RELATION;
@@ -138,28 +180,49 @@ apply (auto)
 done
 
 theorem SemiR_alphabet [simp] :
-assumes assm: "r1 \<in> WF_RELATION" "r2 \<in> WF_RELATION" "COMPOSABLE (\<alpha> r1) (\<alpha> r2)"
+"r1 \<in> WF_RELATION \<and>
+ r2 \<in> WF_RELATION \<and>
+ COMPOSABLE (\<alpha> r1) (\<alpha> r2) \<longrightarrow>
+ \<alpha> (r1 ; r2) = in (\<alpha> r1) \<union> out (\<alpha> r2)"
+apply (simp add: SemiR_def)
+apply (simp add: WF_RELATION_def)
+apply (simp add: WF_ALPHABET_alphabet)
+apply (safe)
+-- {* Subgoal 1 *}
+apply (case_tac "xa \<in> DASHED")
+apply (simp add: SS1_def DASHED_def)
+apply (simp add: out_alphabet_def DASHED_def)
+apply (subgoal_tac "xa \<in> UNDASHED")
+apply (simp add: SS1_def in_alphabet_def UNDASHED_def)
+apply (auto)
+-- {* Subgoal 2 *}
+sorry
+
+(* The following theorem does not seem to proof on my machine. Ask Simon. *)
+
+(*
+theorem SemiR_alphabet [simp] :
+assumes assm:
+  "r1 \<in> WF_RELATION"
+  "r2 \<in> WF_RELATION"
+  "COMPOSABLE (\<alpha> r1) (\<alpha> r2)"
 shows "\<alpha> (r1 ; r2) = in (\<alpha> r1) \<union> out (\<alpha> r2)"
 proof (insert assm, utp_pred_eq_tac)
-  from assm have "\<alpha> r1 \<subseteq> UNDASHED \<union> DASHED" "\<alpha> r2 \<subseteq> UNDASHED \<union> DASHED"
-                 "\<alpha> r1 \<in> WF_ALPHABET" "\<alpha> r2 \<in> WF_ALPHABET"
-    by (auto simp add:WF_RELATION_def)
-  with assm show "(SS1 ` \<alpha> r1 \<union> SS2 ` \<alpha> r2) - dash ` out (\<alpha> r1) = in (\<alpha> r1) \<union> out (\<alpha> r2)"
-    apply(auto simp add:COMPOSABLE_def)
-    apply(simp add: dash_def in_alphabet_def UNDASHED_def)
-    apply(simp add: dash_def out_alphabet_def DASHED_def)
+  from assm have
+    "\<alpha> r1 \<subseteq> UNDASHED \<union> DASHED"
+    "\<alpha> r2 \<subseteq> UNDASHED \<union> DASHED"
+    "\<alpha> r1 \<in> WF_ALPHABET"
+    "\<alpha> r2 \<in> WF_ALPHABET"
+      by (auto simp add: WF_RELATION_def)
+
+  with assm show
+    "(SS1 ` \<alpha> r1 \<union> SS2 ` \<alpha> r2) - dash ` out (\<alpha> r1) = in (\<alpha> r1) \<union> out (\<alpha> r2)"
+      apply (auto simp add: COMPOSABLE_def)
+      apply (simp add: dash_def in_alphabet_def UNDASHED_def)
+      apply (simp add: dash_def out_alphabet_def DASHED_def)
   done
 qed
-
-
-theorem SkipR_alphabet [simp]:
-"\<lbrakk> a \<in> WF_ALPHABET; a \<subseteq> UNDASHED \<rbrakk> \<Longrightarrow> \<alpha> (\<Pi> a) = a \<union> dash ` a"
- by (simp add: SkipR_def)
-
-
-(***********************)
-(* REVIEWED UNTIL HERE *)
-(***********************)
+*)
 
 subsubsection {* Closure Theorems *}
 
@@ -174,9 +237,12 @@ apply (simp add: CondR_def)
 apply (simp add: WF_RELATION_def WF_CONDITION_def)
 done
 
-theorem SemiR_closure [simp, eval]:
-  assumes assm: "r1 \<in> WF_RELATION" "r2 \<in> WF_RELATION" "COMPOSABLE (\<alpha> r1) (\<alpha> r2)"
-  shows  "r1 ; r2 \<in> WF_RELATION"
+theorem SemiR_closure [simp]:
+assumes assm:
+  "r1 \<in> WF_RELATION"
+  "r2 \<in> WF_RELATION"
+  "COMPOSABLE (\<alpha> r1) (\<alpha> r2)"
+shows "r1 ; r2 \<in> WF_RELATION"
 proof -
   from assm have "r1 ; r2 \<in> WF_ALPHA_PREDICATE"
     by (utp_pred_eq_tac)
@@ -214,24 +280,48 @@ apply (auto)
 -- {* TODO: See if the proof of the subgoals can be automated. *}
 oops
 
-thm COMPOSABLE_def
+theorem SemiR_assoc:
+"\<lbrakk>r1 \<in> WF_RELATION;
+ r2 \<in> WF_RELATION;
+ r3 \<in> WF_RELATION;
+ COMPOSABLE (\<alpha> r1) (\<alpha> r2);
+ COMPOSABLE (\<alpha> r2) (\<alpha> r3)\<rbrakk> \<Longrightarrow>
+ r1 ; (r2 ; r3) = (r1 ; r2) ; r3"
+apply (subgoal_tac "r2 ; r3 \<in> WF_RELATION");
+apply (subgoal_tac "r1 ; r2 \<in> WF_RELATION");
+apply (subgoal_tac "COMPOSABLE (\<alpha> r1) (\<alpha> (r2 ; r3))")
+apply (subgoal_tac "COMPOSABLE (\<alpha> (r1 ; r2)) (\<alpha> r3)")
+apply (simp add: SemiR_def)
+apply (simp_all)
+oops
 
-theorem semi_assoc:
- assumes assm: "p \<in> WF_RELATION" "q \<in> WF_RELATION" "r \<in> WF_RELATION"
-               "COMPOSABLE (\<alpha> p) (\<alpha> q)" "COMPOSABLE (\<alpha> q) (\<alpha> r)"
- shows "p ; (q ; r) = (p ; q) ; r"
+(* The following theorem does not seem to proof on my machine. Ask Simon. *)
+
+(*
+theorem SemiR_assoc:
+assumes assm:
+  "r1 \<in> WF_RELATION"
+  "r2 \<in> WF_RELATION"
+  "r3 \<in> WF_RELATION"
+  "COMPOSABLE (\<alpha> r1) (\<alpha> r2)"
+  "COMPOSABLE (\<alpha> r2) (\<alpha> r3)"
+shows "r1 ; (r2 ; r2) = (r1 ; r2) ; r3"
 proof -
-  from assm have r1:"q ; r \<in> WF_RELATION" "p ; q \<in> WF_RELATION"
-    by (auto)
+  from assm have r1 :
+    "r1 ; r2 \<in> WF_RELATION"
+    "r2 ; r3 \<in> WF_RELATION"
+      by (simp_all)
 
-  from assm have r2:"COMPOSABLE (\<alpha> p) (\<alpha> (q ; r))" "COMPOSABLE (\<alpha> (p ; q)) (\<alpha> r)"
-    by(auto elim!:COMPOSABLE_elim)    
+  from assm have r2 :
+    "COMPOSABLE (\<alpha> p) (\<alpha> (q ; r))"
+    "COMPOSABLE (\<alpha> (p ; q)) (\<alpha> r)"
+      by (auto elim! : COMPOSABLE_elim)
 
   from r1 r2 assm show ?thesis
     apply(utp_pred_eq_tac)
     apply(safe)
   sorry
 qed
-
+*)
 end
 end
