theories/generic/utp_alphabet.thy
@@ -40,53 +40,133 @@ definition COMPOSABLE ::
  a2 \<in> WF_ALPHABET\<rbrakk> \<Longrightarrow>
  COMPOSABLE a1 a2 \<longleftrightarrow> (out a1) = dash ` (in a2)"
 
+subsection {* Proof Support *}
+
+theorems utp_alphabet_simps =
+  UNDASHED_def
+  DASHED_def
+  DASHED_TWICE_def
+  COMPOSABLE_def
+  in_alphabet_def
+  out_alphabet_def
+
 subsection {* Theorems *}
 
-theorem WF_ALPHABET_in [simp,intro] :
+subsubsection {* Closure Theorems *}
+
+theorem WF_ALPHABET_empty [simp] :
+"{} \<in> WF_ALPHABET"
+apply (simp add: WF_ALPHABET_def)
+done
+
+theorem WF_ALPHABET_insert [simp] :
+"\<lbrakk>a \<in> WF_ALPHABET\<rbrakk> \<Longrightarrow>
+ (insert x a) \<in> WF_ALPHABET"
+apply (simp add: WF_ALPHABET_def)
+done
+
+theorem WF_ALPHABET_union [simp] :
+"\<lbrakk>a1 \<in> WF_ALPHABET;
+ a2 \<in> WF_ALPHABET\<rbrakk> \<Longrightarrow>
+ a1 \<union> a2 \<in> WF_ALPHABET"
+apply (simp add: WF_ALPHABET_def)
+done
+
+theorem WF_ALPHABET_inter [simp] :
+"\<lbrakk>a1 \<in> WF_ALPHABET;
+ a2 \<in> WF_ALPHABET\<rbrakk> \<Longrightarrow>
+ a1 \<inter> a2 \<in> WF_ALPHABET"
+apply (simp add: WF_ALPHABET_def)
+done
+
+theorem WF_ALPHABET_diff [simp] :
+"\<lbrakk>a1 \<in> WF_ALPHABET;
+ a2 \<in> WF_ALPHABET\<rbrakk> \<Longrightarrow>
+ a1 - a2 \<in> WF_ALPHABET"
+apply (simp add: WF_ALPHABET_def)
+done
+
+theorem WF_ALPHABET_subset [intro] :
+"\<lbrakk>a \<in> WF_ALPHABET; b \<subseteq> a\<rbrakk> \<Longrightarrow>
+ b \<in> WF_ALPHABET"
+apply (simp add: WF_ALPHABET_def)
+apply (simp add: finite_subset)
+done
+
+theorem WF_ALPHABET_image [simp] :
+"\<lbrakk>a \<in> WF_ALPHABET\<rbrakk> \<Longrightarrow>
+ f ` a \<in> WF_ALPHABET"
+apply (simp add: WF_ALPHABET_def)
+done
+
+theorem WF_ALPHABET_in [simp, intro] :
 "a \<in> WF_ALPHABET \<Longrightarrow>
  in a \<in> WF_ALPHABET"
 apply (simp add: in_alphabet_def)
 apply (simp add: WF_ALPHABET_def)
 done
 
-theorem WF_ALPHABET_out [simp,intro] :
+theorem WF_ALPHABET_out [simp, intro] :
 "a \<in> WF_ALPHABET \<Longrightarrow>
  out a \<in> WF_ALPHABET"
 apply (simp add: out_alphabet_def)
 apply (simp add: WF_ALPHABET_def)
 done
 
-lemma WF_ALPHABET_union [intro] :
-"\<lbrakk> a \<in> WF_ALPHABET ; b \<in> WF_ALPHABET \<rbrakk> \<Longrightarrow> a \<union> b \<in> WF_ALPHABET"
-  by (simp add:WF_ALPHABET_def)
+subsection {* Simon's Theorems *}
 
-lemma COMPOSABLE_intro[intro!]: "\<lbrakk> a \<in> WF_ALPHABET ; b \<in> WF_ALPHABET ; out a = dash ` in b \<rbrakk> \<Longrightarrow>
-                                COMPOSABLE a b"
-  by (simp add:COMPOSABLE_def)
+theorem COMPOSABLE_intro [intro!] :
+"\<lbrakk>a \<in> WF_ALPHABET;
+ b \<in> WF_ALPHABET;
+ out a = dash ` in b\<rbrakk> \<Longrightarrow>
+ COMPOSABLE a b"
+apply (auto simp: utp_alphabet_simps)
+done
 
-lemma COMPOSABLE_elim[elim]: "\<lbrakk> COMPOSABLE a b ; a \<in> WF_ALPHABET ; b \<in> WF_ALPHABET ; out a = dash ` in b \<Longrightarrow> P \<rbrakk> \<Longrightarrow> P"
-  by (simp add:COMPOSABLE_def)  
+theorem COMPOSABLE_elim [elim] :
+"\<lbrakk>COMPOSABLE a b;
+ a \<in> WF_ALPHABET;
+ b \<in> WF_ALPHABET;
+ out a = dash ` in b \<Longrightarrow> P\<rbrakk> \<Longrightarrow> P"
+apply (auto simp: utp_alphabet_simps)
+done
 
-lemma COMPOSABLE_dest[dest]: "\<lbrakk> COMPOSABLE a b ; a \<in> WF_ALPHABET ; b \<in> WF_ALPHABET \<rbrakk> \<Longrightarrow> out a = dash ` in b"
-  by (simp add:COMPOSABLE_def)  
+theorem COMPOSABLE_dest [dest] :
+"\<lbrakk>COMPOSABLE a b;
+ a \<in> WF_ALPHABET;
+ b \<in> WF_ALPHABET\<rbrakk> \<Longrightarrow>
+ out a = dash ` in b"
+apply (auto simp: utp_alphabet_simps)
+done
 
-lemma in_alphabet_in[simp]: "in (in a) = in a"
-  by (auto simp add: in_alphabet_def)
+theorem in_alphabet_in [simp] :
+"in (in a) = in a"
+apply (auto simp: utp_alphabet_simps)
+done
 
-lemma in_alphabet_out[simp]: "in (out a) = {}"
-  by (auto simp add: in_alphabet_def out_alphabet_def DASHED_def UNDASHED_def)
+theorem in_alphabet_out [simp] :
+"in (out a) = {}"
+apply (auto simp: utp_alphabet_simps)
+done
 
-lemma out_alphabet_out[simp]: "out (out a) = out a"
-  by (auto simp add: out_alphabet_def)
+theorem out_alphabet_out [simp] :
+"out (out a) = out a"
+apply (auto simp: utp_alphabet_simps)
+done
 
-lemma out_alphabet_in[simp]: "out (in a) = {}"
-  by (auto simp add: in_alphabet_def out_alphabet_def DASHED_def UNDASHED_def)
+theorem out_alphabet_in [simp] :
+"out (in a) = {}"
+apply (auto simp: utp_alphabet_simps)
+done
 
-lemma in_alphabet_union[simp]: "in (a \<union> b) = in a \<union> in b"
-  by (auto simp add: in_alphabet_def)
+theorem in_alphabet_union [simp] :
+"in (a \<union> b) = in a \<union> in b"
+apply (auto simp: utp_alphabet_simps)
+done
 
-lemma out_alphabet_union[simp]: "out (a \<union> b) = out a \<union> out b"
-  by (auto simp add: out_alphabet_def)
-
+theorem out_alphabet_union [simp] :
+"out (a \<union> b) = out a \<union> out b"
+apply (auto simp: utp_alphabet_simps)
+done
 end
 end
