theories/utp_sorts.thy
@@ -151,6 +151,24 @@ declare subseteq_def [simp]
 declare subset_def [simp]
 end
 
+subsection {* Function Sorts *}
+
+class FUNCTION_SORT =
+  fixes MkFunc :: "('a \<Rightarrow> 'a) \<Rightarrow> 'a"
+  fixes DestFunc :: "'a \<Rightarrow> ('a \<Rightarrow> 'a)"
+  fixes IsFunc :: "'a \<Rightarrow> bool"
+(* assumes inverse [simp] : "MkFun (DestFun f) = f" *)
+begin
+
+text {* Function Operators *}
+
+definition idv :: 'a where
+"idv = MkFunc id"
+
+definition app :: "'a \<Rightarrow> 'a \<Rightarrow> 'a" where
+"app = DestFunc"
+end
+
 subsection {* Aggregated Sorts *}
 
 class BASIC_SORT =
@@ -159,19 +177,6 @@ class BASIC_SORT =
 class COMPOSITE_SORT =
   BASIC_SORT + PAIR_SORT + SET_SORT
 
-class FUNCTION_SORT = COMPOSITE_SORT +
-  fixes MkFunc   :: "('a \<Rightarrow> 'a) \<Rightarrow> 'a"
-  fixes DestFunc :: "'a \<Rightarrow> ('a \<Rightarrow> 'a)"
-  fixes IsFunc   :: "'a \<Rightarrow> bool"
-begin
-
-subsubsection {* Function Operators *}
-definition idv :: 'a where
-"idv = MkFunc id"
-
-definition app :: "'a \<Rightarrow> 'a \<Rightarrow> 'a" where
-"app = DestFunc"
-
-end
-
+class COMPOSITE_SORT2 =
+  BASIC_SORT + PAIR_SORT + SET_SORT + FUNCTION_SORT
 end
